From30To40/Callset.v
@@ -1,0 +1,105 @@
+From Coq Require Import String ZArith Eqdep_dec.
+
+From Vyper Require Import Config Calldag L10.Base CheckArith.Builtins.
+From Vyper Require L30.AST L40.AST L30.Callset L40.Callset.
+
+From Vyper.From30To40 Require Import Translate.
+
+
+Local Ltac rr
+:= repeat (rewrite FSet.union_ok
+        || rewrite FSet.add_ok
+        || rewrite FSet.empty_ok
+        || rewrite FSet.singleton_iff
+        || rewrite Bool.andb_true_l
+        || rewrite Bool.andb_true_r
+        || rewrite Bool.andb_false_l
+        || rewrite Bool.andb_false_r
+        || rewrite Bool.orb_true_l
+        || rewrite Bool.orb_true_r
+        || rewrite Bool.orb_false_l
+        || rewrite Bool.orb_false_r).
+
+(** After translation, the callsets are the same. *)
+Lemma callset_translate_small_stmt {C: VyperConfig}
+                                   (B: Builtins.builtin_names_config)
+                                   (ss: L30.AST.small_stmt)
+                                   (l: list L40.AST.stmt)
+                                   (E: translate_small_stmt B ss = inr l)
+                                   (x: string):
+  let _ := string_set_impl in
+  FSet.has (L40.Callset.stmt_list_callset l) x
+   =
+  FSet.has (L30.Callset.small_stmt_callset ss) x.
+Proof.
+destruct ss; cbn in *; inversion E; subst; cbn; rr; try easy;
+  [ destruct string_dec; trivial | ];
+  unfold Translate.var_range;
+  remember (N.to_nat args_count) as k; clear Heqk;
+  induction k; cbn; rr; trivial;
+  apply IHk.
+Qed.
+
+Lemma callset_translate_stmt {C: VyperConfig}
+                             (B: Builtins.builtin_names_config)
+                             (s: L30.AST.stmt)
+                             (l: list L40.AST.stmt)
+                             (E: translate_stmt B s = inr l)
+                             (x: string):
+  let _ := string_set_impl in
+  FSet.has (L40.Callset.stmt_list_callset l) x
+   =
+  FSet.has (L30.Callset.stmt_callset s) x.
+Proof.
+cbn. revert l E. induction s; intros; cbn; rr.
+{ (* small *) cbn in E. apply (callset_translate_small_stmt B). exact E. }
+{ (* if-else *)
+  cbn in E. rename s1 into yes. rename s2 into no.
+  destruct (translate_stmt B yes) as [err | yes']. { discriminate. }
+  destruct (translate_stmt B no) as [err | no']. { discriminate. }
+  inversion E; subst; clear E.
+  assert (IHyes := IHs1 yes' eq_refl). clear IHs1.
+  assert (IHno := IHs2 no' eq_refl). clear IHs2.
+  unfold Callset.stmt_list_callset. rr.
+  cbn. rr.
+  rewrite Bool.orb_comm.
+  f_equal. { apply IHyes. } apply IHno.
+}
+{ (* loop *)
+  (* both "cbn in E" and "simpl in E" hang up *)
+  unfold translate_stmt in E. fold translate_stmt in E.
+  destruct (Z_of_uint256 count =? 0)%Z. { discriminate. }
+  destruct (translate_stmt B s) as [err | body]. { discriminate. }
+  assert (IHbody := IHs body eq_refl). clear IHs.
+  (* here "inversion E" hangs up but this remember helps *)
+  remember (AST.Switch
+         (AST.BuiltinCall (builtin_name_uint256_lt B)
+            (AST.LocalVar var :: AST.Const (uint256_of_Z (2 ^ 256 - Z_of_uint256 count + 1)) :: nil))
+         (AST.Case zero256
+            (AST.Block
+               (AST.SmallStmt
+                  (AST.Abort (AbortException (uint256_of_Z (Z_of_string "loop range overflows")))) :: nil))
+          :: nil)
+         (Some
+            (AST.Block
+               (AST.SmallStmt
+                  (AST.Assign var
+                     (AST.BuiltinCall (builtin_name_uint256_add B) (AST.LoopOffset :: AST.LoopCursor :: nil)))
+                :: body))) :: nil)%list as l'.
+  inversion E; subst; clear E.
+  cbn. rr. apply IHbody.
+}
+(* semicolon *)
+cbn in E.
+destruct (translate_stmt B s1) as [err | t1]. { discriminate. }
+destruct (translate_stmt B s2) as [err | t2]. { discriminate. }
+inversion E; subst; clear E.
+unfold Callset.stmt_list_callset. rr.
+cbn. rr.
+assert (IH1 := IHs1 t1 eq_refl). clear IHs1.
+assert (IH2 := IHs2 t2 eq_refl). clear IHs2.
+rewrite<- IH1. rewrite<- IH2. clear s1 s2 IH1 IH2.
+induction t1; intros; cbn; rr. { easy. }
+rewrite<- Bool.orb_assoc. f_equal.
+apply IHt1.
+Qed.
