From30To40/FunCtx.v
@@ -1,0 +1,324 @@
+From Coq Require Import ZArith NArith String List.
+
+From Vyper Require Import Config NaryFun Calldag.
+From Vyper Require Map.
+From Vyper.L30 Require AST Descend.
+From Vyper.L40 Require AST Descend.
+From Vyper.CheckArith Require Import Builtins.
+
+From Vyper.L10 Require Import Base.
+
+From Vyper.From30To40 Require Import Translate Callset.
+
+
+Local Open Scope list_scope.
+
+Fixpoint translate_decl_alist {C: VyperConfig}
+                              (B: builtin_names_config)
+                              (decls: list (string * L30.AST.decl))
+: string + list (string * L40.AST.decl)
+:= match decls with
+   | nil => inr nil
+   | (_, L30.AST.StorageVarDecl _) :: rest => translate_decl_alist B rest
+   | (name, L30.AST.FunDecl _ nargs body) :: rest =>
+        match translate_stmt B body with
+        | inl err => inl err
+        | inr body' =>
+            match translate_decl_alist B rest with
+            | inl err => inl err
+            | inr rest' => inr ((name, L40.AST.FunDecl name nargs (L40.AST.Block body')) :: rest')
+            end
+        end
+   end.
+
+Local Lemma translate_decl_alist_no_new_names {C: VyperConfig}
+                                              (B: builtin_names_config)
+                                              (decls: list (string * L30.AST.decl))
+                                              (decls': list (string * L40.AST.decl))
+                                              (Ok: translate_decl_alist B decls = inr decls')
+                                              (name: string):
+  In name (map fst decls') -> In name (map fst decls).
+Proof.
+revert decls' Ok. induction decls; intros decls' Ok H.
+{ cbn in Ok. inversion Ok. now subst. }
+destruct a as (n, d). cbn in *.
+destruct d.
+{ (* storage var *) right. apply (IHdecls _ Ok H). }
+destruct (translate_stmt B body) as [err|body']. { discriminate. }
+remember (translate_decl_alist B decls) as t_decls.
+destruct t_decls as [err | t_decls]. { discriminate. }
+inversion Ok. subst. clear Ok.
+destruct H. { now left. }
+right. now apply (IHdecls _ eq_refl).
+Qed.
+
+Lemma translate_decl_alist_ok {C: VyperConfig}
+                              (B: builtin_names_config)
+                              (decls: list (string * L30.AST.decl))
+                              (DeclsNoDup: List.NoDup (List.map fst decls))
+                              (decls': list (string * L40.AST.decl))
+                              (Ok: translate_decl_alist B decls = inr decls')
+                              (name: string):
+  match Map.alist_lookup string_dec decls name with
+  | None | Some (L30.AST.StorageVarDecl _) => Map.alist_lookup string_dec decls' name = None
+  | Some (L30.AST.FunDecl _ nargs body) =>
+      match translate_stmt B body with
+      | inl _ => False
+      | inr body' => Map.alist_lookup string_dec decls' name =
+                        Some (L40.AST.FunDecl name nargs (L40.AST.Block body'))
+      end
+  end.
+Proof.
+revert decls' Ok. induction decls; intros. { cbn in *. now inversion Ok. }
+cbn. destruct a as (key, value).
+cbn in DeclsNoDup. inversion DeclsNoDup. subst.
+assert (IH := IHdecls H2). clear IHdecls.
+cbn in Ok.
+destruct (string_dec name key) as [E|NE].
+{
+  destruct value.
+  { (* storage var *)
+    subst.
+    apply Map.alist_lookup_not_in.
+    intro Hkey.
+    now apply (translate_decl_alist_no_new_names B decls decls') in Hkey.
+  }
+  destruct (translate_stmt B body) as [err|body']. { discriminate. }
+  remember (translate_decl_alist B decls) as t_decls.
+  destruct t_decls. { discriminate. }
+  inversion Ok. subst. clear Ok.
+  cbn. now destruct string_dec.
+}
+destruct value.
+{ (* storage var *) now apply IH. }
+destruct (translate_stmt B body). { discriminate. }
+remember (translate_decl_alist B decls) as t_decls.
+destruct t_decls. { discriminate. }
+inversion Ok. subst. clear Ok.
+cbn. destruct (string_dec name key). { contradiction. }
+apply (IH _ eq_refl).
+Qed.
+
+Local Lemma translate_calldag_depthmap_ok {C: VyperConfig}
+                                          (B: builtin_names_config)
+                                          (name: string)
+                                          (cd: L30.Descend.calldag)
+                                          (d: list (string * L40.AST.decl)):
+   let _ := string_map_impl in
+   forall E: translate_decl_alist B (Map.items (cd_decls cd)) = inr d,
+   match Map.lookup (Map.of_alist d) name with
+   | Some decl =>
+       match cd_depthmap cd name with
+       | Some x =>
+           let H := string_set_impl in
+           FSet.for_all (Callset.decl_callset decl)
+             (fun callee : string =>
+              match cd_depthmap cd callee with
+              | Some y => y <? x
+              | None => false
+              end) = true
+       | None => False
+       end
+   | None => True
+   end.
+Proof.
+intros map_impl E. unfold map_impl in *. clear map_impl.
+remember (Map.lookup _ name) as m. symmetry in Heqm.
+destruct m as [f|]. 2:{ trivial. }
+rewrite Map.of_alist_ok in Heqm.
+
+assert (D := cd_depthmap_ok cd name).
+assert (F := translate_decl_alist_ok B
+                                     (Map.items (cd_decls cd))
+                                     (Map.items_nodup (cd_decls cd))
+                                     d E name).
+rewrite<- Map.items_ok in F.
+destruct (Map.lookup (cd_decls cd) name). 2:{ now rewrite F in Heqm. }
+destruct (cd_depthmap cd name). 2:assumption.
+rewrite FSet.for_all_ok. rewrite FSet.for_all_ok in D.
+intros x H.
+destruct d0; rewrite Heqm in F. { discriminate. }
+cbn in D.
+remember (translate_stmt B body) as body'. destruct body'. { contradiction. }
+inversion F. subst. clear F.
+cbn in H.
+rewrite (callset_translate_stmt B _ _ (eq_sym Heqbody')) in H.
+apply (D x H).
+Qed.
+
+Definition translate_calldag {C: VyperConfig} (B: builtin_names_config) (cd: L30.Descend.calldag)
+: string + L40.Descend.calldag
+:= let _ := string_map_impl in
+   match translate_decl_alist B (Map.items (cd_decls cd)) as cd' return _ = cd' -> _ with
+   | inl err => fun _ => inl err
+   | inr d => fun E => inr
+     {| cd_decls := Map.of_alist d
+      ; cd_depthmap := cd_depthmap cd
+      ; cd_depthmap_ok name := translate_calldag_depthmap_ok B name cd d E
+     |}
+   end eq_refl.
+
+
+(***************************************************************************************************)
+
+Section FunCtx1.
+  Context {C: VyperConfig}
+          {bound: nat}
+          {cd30: L30.Descend.calldag}
+          {cd40: L40.Descend.calldag}
+          (B: builtin_names_config)
+          (ok: translate_calldag B cd30 = inr cd40).
+
+  Lemma translate_fun_ctx_depthmap (name: string):
+    cd_depthmap cd40 name
+     =
+    cd_depthmap cd30 name.
+  Proof.
+  destruct cd30.
+  unfold translate_calldag in ok.
+  cbn in *.
+  remember (fun d (E : translate_decl_alist B (Map.items cd_decls) = inr d) =>
+         inr
+           {|
+             cd_decls := Map.of_alist d;
+             cd_depthmap := cd_depthmap;
+             cd_depthmap_ok :=
+               fun name : string =>
+               translate_calldag_depthmap_ok B name
+                 {|
+                   cd_decls := cd_decls; cd_depthmap := cd_depthmap; cd_depthmap_ok := cd_depthmap_ok
+                 |} d E
+           |}) as good_branch.
+  assert (K: forall (d40: list (string * L40.AST.decl))
+                    (E: translate_decl_alist B (Map.items cd_decls) = inr d40),
+               good_branch d40 E = inr cd40
+                ->
+               Calldag.cd_depthmap cd40 name = cd_depthmap name).
+  {
+    intros. subst.
+    inversion H. now subst.
+  }
+  clear Heqgood_branch.
+  destruct (translate_decl_alist B (Map.items cd_decls)) as [|d40]. { discriminate. }
+  apply (K d40 eq_refl ok).
+  Qed.
+
+  Lemma translate_fun_ctx_declmap (name: string):
+    match cd_declmap cd30 name with
+    | Some (L30.AST.FunDecl n nargs body) =>
+        Some (translate_stmt B body)
+    | _ => None
+    end
+     =
+    match cd_declmap cd40 name with
+    | Some (L40.AST.FunDecl _ _ (L40.AST.Block stmts)) => Some (inr stmts)
+    | None => None
+    end.
+  Proof.
+  destruct cd30.
+  unfold translate_calldag in ok.
+  cbn in *.
+  remember (fun d (E: translate_decl_alist B (Map.items cd_decls) = inr d) =>
+         inr
+           {|
+             cd_decls := Map.of_alist d;
+             cd_depthmap := cd_depthmap;
+             cd_depthmap_ok :=
+               fun name : string =>
+               translate_calldag_depthmap_ok B name
+                 {|
+                   cd_decls := cd_decls; cd_depthmap := cd_depthmap; cd_depthmap_ok := cd_depthmap_ok
+                 |} d E
+           |}) as good_branch.
+  unfold cd_declmap. cbn.
+  assert (K: forall (d40: list (string * L40.AST.decl))
+                    (E: translate_decl_alist B (Map.items cd_decls) = inr d40),
+               good_branch d40 E = inr cd40
+                ->
+               let _ := string_map_impl in
+               match Map.lookup cd_decls name with
+               | Some (L30.AST.FunDecl _ _ body) => Some (translate_stmt B body)
+               | _ => None
+               end
+                =
+               match Map.lookup (Calldag.cd_decls cd40) name with
+               | Some (AST.FunDecl _ _ (AST.Block stmts)) => Some (inr stmts)
+               | None => None
+               end).
+  {
+    intros. subst.
+    inversion H. subst.
+    cbn.
+    clear H ok.
+    assert (M := translate_decl_alist_ok B (Map.items (cd_decls))
+                                         (Map.items_nodup _) _ E name).
+    rewrite Map.of_alist_ok.
+    rewrite<- Map.items_ok in M.
+    destruct (Map.lookup cd_decls name). 2:{ now rewrite M. }
+    destruct d. { now rewrite M. }
+    destruct (translate_stmt B body). { contradiction. }
+    now rewrite M.
+  }
+  clear Heqgood_branch.
+  destruct (translate_decl_alist B (Map.items cd_decls)). { discriminate. }
+  apply (K _ eq_refl ok).
+  Qed.
+End FunCtx1.
+
+Section FunCtx2.
+  Context {C: VyperConfig}
+          {bound: nat}
+          {cd30: L30.Descend.calldag}
+          (fc: fun_ctx cd30 bound)
+          {cd40: L40.Descend.calldag}
+          (B: builtin_names_config)
+          (ok: translate_calldag B cd30 = inr cd40)
+          (NotVar: forall x: string,
+                     fun_decl fc <> L30.AST.StorageVarDecl x).
+
+  Local Lemma translate_fun_ctx_fun_decl_helper:
+    cd_declmap cd40 (fun_name fc) <> None.
+  Proof.
+  intro E.
+  assert (Ok := fun_decl_ok fc).
+  assert (M := translate_fun_ctx_declmap B ok (fun_name fc)).
+  rewrite Ok in M.
+  rewrite E in M.
+  destruct (fun_decl fc). 2:discriminate.
+  exact (NotVar name eq_refl).
+  Qed.
+
+  Definition cached_translated_decl
+  := match cd_declmap cd40 (fun_name fc)
+     as d' return _ = d' -> _
+     with
+     | Some f => fun _ => f
+     | None => fun E =>
+          False_rect _ (translate_fun_ctx_fun_decl_helper E)
+     end eq_refl.
+
+  Local Lemma translate_fun_ctx_decl_ok:
+    cd_declmap cd40 (fun_name fc) 
+     =
+    Some cached_translated_decl.
+  Proof.
+  assert (D := fun_decl_ok fc).
+  unfold cached_translated_decl.
+  remember translate_fun_ctx_fun_decl_helper as foo. clear Heqfoo. revert foo.
+  destruct (cd_declmap cd40 (fun_name fc)). { trivial. }
+  intro. contradiction.
+  Qed.
+
+  Definition translate_fun_ctx
+  : fun_ctx cd40 bound
+  := let name := fun_name fc in
+     {| fun_name := name
+      ; fun_depth := fun_depth fc
+      ; fun_depth_ok :=
+          eq_trans (translate_fun_ctx_depthmap B ok name)
+                   (fun_depth_ok fc)
+      ; fun_decl := cached_translated_decl
+      ; fun_decl_ok := translate_fun_ctx_decl_ok
+      ; fun_bound_ok := fun_bound_ok fc
+     |}.
+End FunCtx2.
