From30To40/Translate.v
@@ -1,0 +1,166 @@
+From Coq Require Import ZArith NArith String.
+
+From Vyper Require Import Config NaryFun.
+From Vyper Require L30.AST L40.AST.
+From Vyper.CheckArith Require Import Builtins.
+
+From Vyper.L10 Require Import Base.
+
+Local Open Scope string_scope.
+Local Open Scope list_scope.
+
+
+Definition BuiltinsSupportSload {C: VyperConfig}
+                                (B: builtin_names_config)
+                                (builtins: string -> option builtin)
+:= match builtins (builtin_name_sload B) with
+   | Some (existT _ 1 sload) =>
+       forall (w: world_state) (name: string),
+         match sload w (string_hash name) with
+         | (w', ExprAbort _) => False
+         | (w', ExprSuccess val) =>
+               w = w'
+                /\
+               val = match storage_lookup w name with
+                     | Some x => x
+                     | None => zero256
+                     end
+         end
+   | _ => False
+   end.
+
+Definition BuiltinsSupportSstore {C: VyperConfig}
+                                 (B: builtin_names_config)
+                                 (builtins: string -> option builtin)
+:= match builtins (builtin_name_sstore B) with
+   | Some (existT _ 2 sstore) =>
+       forall (w: world_state) (name: string) (value: uint256),
+         match sstore w (string_hash name) value with
+         | (w', ExprAbort _) => False
+         | (w', ExprSuccess _) =>
+               w' = storage_insert w name value
+         end
+   | _ => False
+   end.
+
+Definition BuiltinsSupportStorage {C: VyperConfig}
+                                  (B: builtin_names_config)
+                                  (builtins: string -> option builtin)
+:= BuiltinsSupportSload B builtins /\ BuiltinsSupportSstore B builtins.
+
+
+
+Local Definition var_range {C: VyperConfig} (offset count: N)
+: list L40.AST.expr
+:= let fix var_range' (countdown: nat)
+   := match countdown with
+      | O => nil
+      | S k => cons (L40.AST.LocalVar (offset + count - 1 - N.of_nat k)%N)
+                    (var_range' k)
+      end
+   in var_range' (N.to_nat count).
+
+Local Example var_range_example {C: VyperConfig}:
+  var_range 5 3 = (AST.LocalVar 5 :: AST.LocalVar 6 :: AST.LocalVar 7 :: nil)%list.
+Proof.
+trivial.
+Qed.
+
+Definition translate_small_stmt {C: VyperConfig} (B: builtin_names_config) (ss: L30.AST.small_stmt)
+: string + list L40.AST.stmt
+:= let op_err := "an operator in L30 can't possibly occur after the CheckArith pass"%string in
+   match ss with
+   | L30.AST.Pass => inr nil
+   | L30.AST.Const dst val =>
+      inr ((L40.AST.SmallStmt (L40.AST.Assign dst (L40.AST.Const val))) :: nil)
+   | L30.AST.Copy dst src =>
+      inr ((L40.AST.SmallStmt (L40.AST.Assign dst (L40.AST.LocalVar src))) :: nil)
+   | L30.AST.StorageGet dst name =>
+      inr ((L40.AST.SmallStmt
+              (L40.AST.Assign dst
+                (L40.AST.BuiltinCall
+                  (builtin_name_sload B)
+                  (L40.AST.Const (string_hash name) :: nil)))) :: nil)
+   | L30.AST.StoragePut name src =>
+      inr ((L40.AST.SmallStmt
+              (L40.AST.ExprStmt
+                (L40.AST.BuiltinCall
+                  (builtin_name_sstore B)
+                  (L40.AST.Const (string_hash name) :: L40.AST.LocalVar src :: nil)))) :: nil)
+   | L30.AST.UnOp _ _ _ => inl op_err
+   | L30.AST.PowConstBase _ _ _ => inl op_err
+   | L30.AST.PowConstExp _ _ _ => inl op_err
+   | L30.AST.BinOp _ _ _ _ _ => inl op_err
+   | L30.AST.PrivateCall dst name args_offset args_count =>
+        inr ((L40.AST.SmallStmt
+               (L40.AST.Assign dst
+                 (L40.AST.PrivateCall name (var_range args_offset args_count)))) :: nil)
+   | L30.AST.BuiltinCall dst name args_offset args_count =>
+        inr ((L40.AST.SmallStmt
+               (L40.AST.Assign dst
+                 (L40.AST.BuiltinCall name (var_range args_offset args_count)))) :: nil)
+   | L30.AST.Abort ab =>
+        inr ((L40.AST.SmallStmt (L40.AST.Abort ab)) :: nil)
+   | L30.AST.Return var =>
+        inr ((L40.AST.SmallStmt (L40.AST.Return (L40.AST.LocalVar var))) :: nil)
+   | L30.AST.Raise var =>
+        inr ((L40.AST.SmallStmt (L40.AST.Raise  (L40.AST.LocalVar var))) :: nil)
+   end.
+
+Fixpoint translate_stmt {C: VyperConfig} (B: builtin_names_config) (s: L30.AST.stmt)
+{struct s}
+: string + list L40.AST.stmt
+:= match s with
+   | L30.AST.SmallStmt ss => translate_small_stmt B ss
+   | L30.AST.Semicolon a b =>
+      match translate_stmt B a with
+      | inl err => inl err
+      | inr aa => match translate_stmt B b with
+                  | inl err => inl err
+                  | inr bb => inr (aa ++ bb)
+                  end
+      end
+   | L30.AST.IfElseStmt condvar yes no =>
+      match translate_stmt B yes with
+      | inl err => inl err
+      | inr yes' =>
+          match translate_stmt B no with 
+          | inl err => inl err
+          | inr no' =>
+              inr (L40.AST.Switch (L40.AST.LocalVar condvar)
+                                  (L40.AST.Case zero256 (L40.AST.Block no') :: nil)
+                                  (Some (L40.AST.Block yes')) :: nil)
+          end
+      end
+   | L30.AST.Loop loopvar count body =>
+      let count_z := Z_of_uint256 count in
+      if (count_z =? 0)%Z
+        then inl "zero-count loops are not allowed"
+        else match translate_stmt B body with
+             | inl err => inl err
+             | inr body' =>
+                  inr
+                    (* start_z + count_z - 1 < 2^256
+                        <->
+                       start_z < 2^256 - count_z + 1 *)
+                    (L40.AST.Switch
+                      (L40.AST.BuiltinCall
+                        (builtin_name_uint256_lt B)
+                          (L40.AST.LocalVar loopvar
+                             ::L40.AST.Const (uint256_of_Z (2 ^ 256 - count_z + 1)%Z)
+                             :: nil))
+                      (L40.AST.Case zero256
+                        (L40.AST.Block
+                          (L40.AST.SmallStmt
+                            (L40.AST.Abort
+                              (AbortException (uint256_of_Z (Z_of_string "loop range overflows"))))
+                          :: nil)) :: nil)
+                      (Some
+                        (L40.AST.Block
+                          ((L40.AST.SmallStmt
+                            (L40.AST.Assign loopvar
+                              (L40.AST.BuiltinCall (builtin_name_uint256_add B)
+                                (L40.AST.LoopOffset :: L40.AST.LoopCursor :: nil))))
+                          :: body'))) :: nil)
+             end
+   end.
