NUANCES.md
@@ -51,8 +51,3 @@ The semantics of _uint256_ is defined without requiring only one representation 
 This does not affect the semantics of the language because there's no way to obtain and no way to detect the integers outside of the 0..2<sup>256</sup> range by using the basic operators. However, that could be possible with custom built-in functions.
 
 There's one (fortunately, only one) resulting quirk in the compiler: it is unable to to replace _x ** 1_ with _x_. The reason is, _x ** 1_ is the canonical representation of _x_ and therefore is not identical to _x_, but merely indistinguishable from _x_ by normal means. But the compiled code must produce an identical result.
-
-
-## Zero Values for Missing Storage Variables
-
-What should happen if we try to access a storage variable but it's just not there? It might seem natural to raise an error. But a better way is to just silently assume the variable to be 0. The reason is that any built-in function could, at least in principle, unexpectedly remove the variable from the storage, and the effort required to ensure this does not happen is simply not worth it.
